
\medskip

\[\cos \left(\dfrac{9\pi}{5}\right) = \dfrac{\sqrt 5 + 1}{4} \qquad \text{et} \qquad \dfrac{\pi}{5} = \dfrac{10\pi}{5} - \dfrac{9\pi}{5} = 2\pi - \dfrac{9\pi}{5}\]

Or, pour tout r√©el $x$, on a :
\[\cos \left(2\pi - x\right) = \cos \left(-x\right) \qquad \text{et} \qquad \cos \left(-x\right) = \cos \left(x\right).\]

Donc :
\begin{align*}
\cos \left(\dfrac{\pi}{5}\right) &= \cos \left(2\pi - \dfrac{9\pi}{5}\right) \\
&=  \cos \left(-\dfrac{9\pi}{5}\right) \\
&=  \cos \left ( \dfrac{9\pi}{5}\right) \\
&= \dfrac{\sqrt{5}+1}{4}
\end{align*}

\bigskip

