
\medskip

On veut déterminer $\displaystyle\lim_{x \to + \infty} (-4x + 8)\e^{-x} =\ds\lim _{x \to +\infty} \left (-4x\e^{-x} +8\e^{-x}\right )$.

On sait que :
\[\ds\lim_{x \to +\infty} \e^{-x} = 0 \text{ donc } \ds\lim_{x \to +\infty} 8\e^{-x} = 0,\]

et comme $x\e^{-x} = \dfrac{x}{\e^x}$, d'après le théorème des croissances comparées :
\[\ds\lim_{x \to +\infty} \dfrac{x}{\e^x} = 0 \text{ et } \ds\lim_{x \to +\infty} -4\dfrac{x}{\e^x} = 0.\]

Donc $\ds\lim_{x \to +\infty} \left(-4x\e^{-x} +8\e^{-x}\right) = 0$,
et donc $\displaystyle\lim_{x \to + \infty} (-4x + 8)\e^{-x} =0 $.

\bigskip

