
\medskip

\begin{enumerate}
\item Pour tout $x$ appartenant Ã  $\R$,\\
  $F'(x) = \left (2x+3\right )\times \e^{x} +  \left(x^2 + 3x + 1\right) \times \e^{x}
  = \left (2x+3 + x^2 +3x+1\right ) \e^{x}
  = \left (x^2+5x+4\right ) \e^{x}\\
\phantom{F'(x)} 
 = f(x)$.
  
Donc la fonction $F$ est une primitive de la fonction $f$ sur $\R$.
  
\item $\displaystyle\int_0^1 f(x)\d x
= \left [ F(x)\strut\right ]_{0}^{1} 
= F(1)-F(0)
= \left ( (1+3+1)\e^{1}\right ) - \left ( (0+0+1)\e^{0} \right )
= 5\e - 1$

\end{enumerate}

\bigskip

