
\medskip

\begin{enumerate}
\item $u(t) = \dfrac{7\sqrt{3}}{4}\cos (100t) - \dfrac{7}{4}\sin (100t)
= \dfrac{7}{2} \times \dfrac{\sqrt{3}}{2}\cos (100t) - \dfrac{7}{2}\times \dfrac{1}{2}\sin(100t)\\
\phantom{u(t)}
=  \dfrac{7}{2} \left ( \cos (100t) \times \dfrac{\sqrt{3}}{2} -\sin(100t)\times \dfrac{1}{2}\right )
$

Or $\dfrac{\sqrt{3}}{2}=\cos \left (\dfrac{\pi}{6}\right )$ et $\dfrac{1}{2}= \sin \left (\dfrac{\pi}{6}\right )$.
Donc:

$u(t) = \dfrac{7}{2} \left ( \cos (100t) \cos \left (\dfrac{\pi}{6}\right ) -\sin(100t) \sin\left (\dfrac{\pi}{6}\right )\right )
= \dfrac{7}{2} \cos \left (100t+ \dfrac{\pi}{6}\right )$.

\item Le déphasage $\varphi$ de $u(t)$ est donc égal à $\dfrac{\pi}{6}$.
\end{enumerate}

\bigskip

