
\medskip

On regarde si la fonction $f$ vérifie les conditions requises.

\begin{list}{\textbullet}{}
\item $f(t) = \cos(t) + 2 \sin(t)$ donc
$f'(t)= -\sin(t) +2\cos(t)$ et
$f''(t)= -\cos(t) -2\sin(t)$.

$f''(t)+f(t) = \left (-\cos(t) -2\sin(t)\right ) + \left ( \cos(t) + 2 \sin(t)\right ) = 0$ donc la fonction $f$ est solution de l'équation différentielle $(E)$.

\item $f(t) = \cos(t) + 2 \sin(t)$ donc $f(0)=\cos(0) + 2 \sin(0) = 1$

\item $f'(t)= -\sin(t) +2\cos(t)$  donc $f'(0)= -\sin(0) +2\cos(0) = 2$ 
\end{list}

\medskip

\textbf{Affirmation 4 vraie}

\bigskip

