
\medskip

$z = \dfrac{2 - \text{i}}{1 - 3\text{i}}
= \dfrac{(2-\text{i})(1+3\text{i})}{(1-3\text{i})(1+3\text{i})}
= \dfrac{2-\text{i}+6\text{i} -3\text{i}^2}{1-(3\text{i})^2}
= \dfrac{5+5\text{i}}{10}
= \dfrac{1}{2} + \dfrac{1}{2}\text{i}$

$\left |z\right | = \ds\sqrt{\left (\dfrac{1}{2}\right )^2 + \left (\dfrac{1}{2}\right )^2} 
=\ds\sqrt{\dfrac{1}{4}+ \dfrac{1}{4}}
= \ds\sqrt{\dfrac{2}{4}}
= \dfrac{\sqrt{2}}{2}$

$z = \dfrac{\sqrt{2}}{2} \left ( \dfrac{\sqrt{2}}{2} + \dfrac{\sqrt{2}}{2} \text{i}\right )
= \dfrac{\sqrt{2}}{2} \left ( \cos \dfrac{\pi}{4} + \text{i} \sin \dfrac{\pi}{4}\right )
= \dfrac{\sqrt{2}}{2} \e^{\text{i}\frac{\pi}{4}}$

$z^4 = \left ( \dfrac{\sqrt{2}}{2} \right )^4 \e^{4\times \text{i}\frac{\pi}{4}}
= \dfrac{1}{4} \e^{\text{i} \pi }= -\dfrac{1}{4}$

\medskip

\textbf{Affirmation 5 vraie}
 
\bigskip
 
