
\medskip

\begin{enumerate}
\item On a : $|z| = \sqrt{\left(\sqrt{3}\right)^2 + (- 1)^2} = \sqrt{3 + 1} = \sqrt{4} = 2$ ;

Donc : $z = 2\left(\dfrac{\sqrt{3}}{2} + \text{i} \dfrac{-1}{2}\right) = 2 \left(\cos \frac{-\pi}{6} + \text{i}\sin \frac{-\pi}{6}\right) = 2 \text{e}^{-\text{i}\frac{\pi}{6}}$.

\item Tout d'abord : $z' = -\sqrt{2}\e^{\text{i}\frac{\pi}{4}} = \sqrt{2}\text{e}^{\text{i}\pi}\times \e^{\text{i}\frac{\pi}{4}} = \sqrt{2}\text{e}^{\text{i}\frac{5\pi}{4}}$.

Donc : $\dfrac{z}{z'} = \dfrac{2 \text{e}^{-\text{i}\frac{\pi}{6}}}{\sqrt{2}\text{e}^{\text{i}\frac{5\pi}{4}}} =  \sqrt{2}\text{e}^{\text{i}\left(-\frac{\pi}{6} - \frac{5\pi}{4}\right)} = \sqrt{2}\text{e}^{-\text{i}\left(\frac{17\pi}{12}\right)} = \sqrt{2}\text{e}^{\text{i}\frac{7\pi}{12}}$.
\end{enumerate}

\bigskip

